closer still

Affine/Normalize.lean
@@ -26,11 +26,33 @@ def normalize (e : Lambda) : Lambda :=
   else
     have : e.small_step.count_β < e.count_β := e.small_step_count_β_lt h
     e.small_step.normalize
-
 termination_by e.count_β
 
-@[simp] theorem small_step_count (e : Lambda) (x : ℕ) : e.small_step.count x = e.count x := by sorry
-@[simp] theorem small_step_free (e : Lambda) : e.small_step.free = e.free := by sorry
+@[simp] theorem small_step_count (e : Lambda) (x : ℕ) : e.small_step.count x ≤ e.count x := by
+  match e with
+  | .var x' => simp only [count, le_refl]
+  | .abs x' e => simp only [count, small_step_count e x, ite_le_ite (le_refl 0)]
+  | .app (.var x') e₂ => simp only [count, small_step_count e₂ x, add_le_add_iff_left]
+  | .app (.abs x' e₁) e₂ => simp only [count, small_step, substₑ_count, le_refl]
+  | .app (.app e₁ e₂) e₃ =>
+    simp only [count, small_step, small_step_count]
+    exact add_le_add
+      (add_le_add (e₁.small_step_count x) (e₂.small_step_count x))
+      (e₃.small_step_count x)
+
+@[simp] theorem small_step_free (e : Lambda) : e.small_step.free ⊆ e.free := by
+  match e with
+  | .var x' => simp only [free, Finset.Subset.refl]
+  | .abs x' e =>
+    simp only [free, small_step_free e, Finset.sdiff_subset_sdiff _ (Finset.Subset.refl _)]
+  | .app (.var x') e₂ =>
+    simp only [free, small_step_free e₂, Finset.union_subset_union (Finset.Subset.refl _)]
+  | .app (.abs x' e₁) e₂ => simp only [free, small_step, substₑ_free]
+  | .app (.app e₁ e₂) e₃ =>
+    simp only [count, free, small_step, small_step_count]
+    exact Finset.union_subset_union
+      (Finset.union_subset_union e₁.small_step_free e₂.small_step_free)
+      e₃.small_step_free
 
 @[simp] theorem small_step_is_affine {e : Lambda} (h : e.is_affine) : e.small_step.is_affine := by
   match e with
@@ -38,14 +60,20 @@ termination_by e.count_β
 
   | .abs x e =>
     have ⟨he, hc⟩ := is_affine_of_abs.mp h
-    simp only [small_step, small_step_is_affine he, is_affine_of_abs, small_step_count e x, hc,
-      and_self]
+    simp only [small_step, small_step_is_affine he, is_affine_of_abs, hc,
+      le_trans (small_step_count e x) hc, and_self]
 
   | .app (.var x) e₂ =>
-    simp only [is_affine_of_app, is_affine_of_var, true_and] at h
+    simp only [is_affine_of_app, is_affine_of_var, free, true_and] at h
     have ⟨he₂, hinter⟩ := h
     simp only [small_step, is_affine_of_app, is_affine_of_var, small_step_is_affine he₂, hinter,
-      small_step_free, true_and]
+      small_step_free, free, true_and]
+    by_cases hx : x ∈ e₂.free
+    · simp only [Finset.singleton_ne_empty, Finset.singleton_inter_of_mem hx, and_false] at h
+    · simp only [Finset.singleton_inter_of_not_mem hx, and_true] at h
+      have := Finset.inter_subset_inter (Finset.Subset.refl {x}) (small_step_free e₂)
+      apply Finset.subset_empty.mp
+      simp only [← hinter, this]
 
   | .app (.abs x e₁) e₂ =>
     simp only [is_affine_of_app, is_affine_of_abs] at h
@@ -57,6 +85,15 @@ termination_by e.count_β
     have ⟨⟨he₁, he₂, hfree₁₂⟩, he₃, hfree₁₂₃⟩ := h
     simp only [small_step, is_affine_of_app, small_step_is_affine he₁, small_step_is_affine he₂,
       small_step_is_affine he₃, small_step_free, free, hfree₁₂, hfree₁₂₃, true_and]
+
+    apply And.intro
+    · simp_rw [← Finset.subset_empty, ← hfree₁₂,
+        Finset.inter_subset_inter e₁.small_step_free e₂.small_step_free]
+    · apply Finset.subset_empty.mp
+      rw [← hfree₁₂₃]
+      exact Finset.inter_subset_inter
+        (Finset.union_subset_union e₁.small_step_free e₂.small_step_free)
+        e₃.small_step_free
 
 @[simp] theorem normalize_of_var (x : ℕ) : (var x).normalize = var x := by
   unfold normalize
@@ -71,13 +108,15 @@ termination_by e.count_β
     simp_rw [dif_neg hc, small_step, normalize_of_abs e.small_step]
 termination_by e.count_β
 
-@[simp] theorem normalize_free_eq (e : Lambda) : e.normalize.free = e.free := by
+@[simp] theorem normalize_free_eq (e : Lambda) : e.normalize.free ⊆ e.free := by
   unfold normalize
   simp only [count_β, dif_pos]
   by_cases hc : e.count_β = 0
-  · simp_rw [dif_pos hc]
+  · simp_rw [dif_pos hc, Finset.Subset.refl]
   · have : e.small_step.count_β < e.count_β := small_step_count_β_lt e hc
-    simp_rw [dif_neg hc, normalize_free_eq e.small_step, small_step_free]
+    have h₁ : e.small_step.normalize.free ⊆ e.small_step.free := normalize_free_eq e.small_step
+    have h₂ : e.small_step.free ⊆ e.free := small_step_free e
+    simp_rw [dif_neg hc, Finset.Subset.trans h₁ h₂]
 termination_by e.count_β
 
 @[simp] theorem normalize_affine {e : Lambda} (h : e.is_affine) : e.normalize.is_affine := by
@@ -95,15 +134,12 @@ end Lambda
 
 namespace Affine
 
-def normalize (e : Affine vs) : (vs' : Finset ℕ) × (_ : Affine vs') ×' (vs' = vs) :=
+def normalize (e : Affine vs) : (vs' : Finset ℕ) × (_ : Affine vs') ×' (vs' ⊆ vs) :=
   let e' := e.to_lambda.normalize
-
-  have he'_free_sub : e'.free = vs := by
+  have he'_free_sub : e'.free ⊆ vs := by
     rw [e.free_eq, to_lambda_free_eq e]
     exact Lambda.normalize_free_eq e.to_lambda
-
   have he'_is_affine : e'.is_affine := Lambda.normalize_affine e.to_lambda_is_affine
-
   ⟨e'.free, Affine.of_lambda he'_is_affine, he'_free_sub⟩
 
 end Affine
